refinement: LowComp: revise l_eq_axiom and fix following lemmas
As discussed in several calls, this axiom is not sound due to bad
interactions with subtying and untyped equality, as we recently
discovered for plain functional extensionality.

So, apply a similar fix by making the "domain"--the high-level
computation-- explicit in the conclusion of the axiom.

examples/refinement/LowComp.fst
@@ -22,7 +22,7 @@ open LowStar.Buffer
 open LowStar.BufferOps
 open LowStar.Modifies
 open Mem_eq
-open Relations 
+open Relations
 
 module H = FStar.Monotonic.Heap
 module B = LowStar.Buffer
@@ -73,11 +73,11 @@ let state_as_lstate_put_get h ls bs =
 
 val state_as_lstate_get_put : h:HS.mem -> ls:lstate{well_formed h ls} ->
     Lemma (state_as_lstate h ls (lstate_as_state h ls) == h)
-let state_as_lstate_get_put h ls = 
+let state_as_lstate_get_put h ls =
     let (b1, b2) = ls in
-    let s1 = B.get h b1 0 in 
-    let s2 = B.get h b2 0 in 
-    
+    let s1 = B.get h b1 0 in
+    let s2 = B.get h b2 0 in
+
     let h1 = g_upd b1 0 s1 h in
     let l1 = g_upd_preserves_live h b1 b2 s1 in
     let h2 = g_upd b2 0 s2 h1 in
@@ -85,10 +85,9 @@ let state_as_lstate_get_put h ls =
 
     let p1 = get_upd_eq h b1 0 s1 in
     assert (h1 == h);
-    let p2 = get_upd_eq h b2 0 s2 in 
+    let p2 = get_upd_eq h b2 0 s2 in
     assert (h2 == h);
     ()
-    
 
 val state_as_lstate_put_put : h:HS.mem -> ls:lstate{well_formed h ls} -> bs1:state -> bs2:state ->
     Lemma (state_as_lstate h ls bs2 == state_as_lstate (state_as_lstate h ls bs1) ls bs2)
@@ -139,8 +138,12 @@ let lcomp (a : Type) pre post (c : comp_p a pre post) =
 //Rather than get into trouble with applying `c` directly in a context
 //where we have to think about the VC of the continuation,
 //let's factor this into a `run`, which makes things a lot more predictable
+<<<<<<< HEAD
 let run_high #a #wp (c:comp_wp a wp) (s0:_{wp s0 (fun _ -> True)}) : Tot (a * state) =
   c s0
+=======
+let run_high #a #wp (c:comp_wp a wp) (s0:_{wp s0 (fun _ -> True)}) : Tot (a * state) = c s0
+>>>>>>> refinement: LowComp: revise l_eq_axiom and fix following lemmas
 
 type lwp a = lstate -> (mem -> (a * mem -> Type) -> Type)
 
@@ -175,9 +178,18 @@ let l_eq #a (#wp1:hwp_mon a) (#c1:comp_wp a wp1) (lc1: lcomp_wp a wp1 c1)
          (#wp2:hwp_mon a) (#c2:comp_wp a wp2) (lc2 : lcomp_wp a wp2 c2) =
   lwp_eq (as_lwp c1) (as_lwp c2)
 
+assume val on_wp (#a:Type) (#wp : hwp_mon a) (c : comp_wp a wp) (lc : lcomp_wp a wp c) : lcomp_wp a wp c
 
+(* unused for now *)
+assume val on_wp_idem (#a:Type) (#wp : hwp_mon a) (c : comp_wp a wp) (lc : lcomp_wp a wp c)
+  : Lemma (on_wp c (on_wp c lc) == lc)
 let l_eq_refl #a (#wp:hwp_mon a) (#c:comp_wp a wp) (lc: lcomp_wp a wp c) : Lemma (l_eq lc lc) = ()
 
+<<<<<<< HEAD
+let l_eq_refl #a (#wp:hwp_mon a) (#c:comp_wp a wp) (lc: lcomp_wp a wp c) : Lemma (l_eq lc lc) = ()
+
+=======
+>>>>>>> refinement: LowComp: revise l_eq_axiom and fix following lemmas
 let l_eq_symm #a (#wp1:hwp_mon a) (#c1:comp_wp a wp1) (lc1: lcomp_wp a wp1 c1)
                  (#wp2:hwp_mon a) (#c2:comp_wp a wp2) (lc2 : lcomp_wp a wp2 c2) (_ : squash (l_eq lc1 lc2)) : Lemma (l_eq lc2 lc1) = ()
 
@@ -186,7 +198,7 @@ let l_eq_trans #a (#wp1:hwp_mon a) (#c1:comp_wp a wp1) (lc1:lcomp_wp a wp1 c1)
                   (#wp3:hwp_mon a) (#c3:comp_wp a wp2) (lc3:lcomp_wp a wp2 c2)
                   (_ : squash (l_eq lc1 lc2)) (_ : squash (l_eq lc2 lc3)) : Lemma (l_eq lc1 lc3) = ()
 
-let uncurry3 #a #b #c (r : #a -> #b -> c -> #a -> #b -> c -> Type) : relation (a * b * c) = 
+let uncurry3 #a #b #c (r : #a -> #b -> c -> #a -> #b -> c -> Type) : relation (a * b * c) =
   fun (x, y, z) (x', y', z') -> r x y z x' y' z'
 
 let l_eq' #a : relation (wp:hwp_mon a & c:comp_wp a wp & lcomp_wp a wp c) =
@@ -196,13 +208,12 @@ let l_eq' #a : relation (wp:hwp_mon a & c:comp_wp a wp & lcomp_wp a wp c) =
 
 instance l_eq_equiv #a : equiv (l_eq' #a) = { refl'  = (fun x -> ());
                                               symm'  = (fun x y p -> ());
-                                              trans' = (fun x y z p1 p2 -> ()); } 
-
-
+                                              trans' = (fun x y z p1 p2 -> ()); }
 
 assume val l_eq_axiom : (#a:Type) -> (#wp1:hwp_mon a) -> (#c1:comp_wp a wp1) -> (lc1: lcomp_wp a wp1 c1) ->
                         (#wp2:hwp_mon a) -> (#c2:comp_wp a wp2) -> (lc2 : lcomp_wp a wp2 c2) ->
-                        Lemma (requires (l_eq lc1 lc2)) (ensures (lc1 === lc2))
+                        Lemma (requires (l_eq lc1 lc2))
+                              (ensures (on_wp c1 lc1 === on_wp c2 lc2))
 
 // Guido
    let gh1 : comp_wp int (fun _ _ -> False) = return_elab 1
@@ -508,7 +519,7 @@ let morph_return #a (wp : hwp_mon a) (c : comp_wp a wp) (x : a) :
   Lemma
     (requires (c === return_elab x))
     (ensures (return_inv c x;
-              morph wp c == lreturn x)) =
+              on_wp c (morph wp c) == on_wp c (lreturn x))) =
   let p = return_inv c x in
   assert (subsumes (return_wp x) wp);
   assert (l_eq #a
@@ -528,7 +539,7 @@ let morph_read (wp : hwp_mon mint) (c : comp_wp mint wp) (i : nat{i < 2}) :
   Lemma
     (requires (c === hread_elab i))
     (ensures (read_inv c i;
-              morph wp c == lread' i)) =
+              on_wp c (morph wp c) == on_wp c (lread' i))) =
   let p = read_inv c i in
   assert (subsumes (read_wp i) wp);
   assert (l_eq #mint
@@ -543,7 +554,7 @@ let morph_write (wp : hwp_mon unit) (c : comp_wp unit wp) (i : nat{i < 2}) (v : 
   Lemma
     (requires (c === hwrite_elab i v))
     (ensures (write_inv c i v;
-              morph wp c == lwrite' i v)) =
+              on_wp c (morph wp c) == on_wp c (lwrite' i v))) =
   let p = write_inv c i in
   assert (subsumes (write_wp i v) wp);
   assert (l_eq #unit
@@ -559,7 +570,7 @@ let morph_bind #a #b (wp1 : hwp_mon a) (c1 : comp_wp a wp1)
     (wp : hwp_mon b) (c : comp_wp b wp) :
   Lemma (requires (c === bind_elab c1 c2))
         (ensures (bind_inv c1 c2 c;
-                  morph wp c == lbind (morph wp1 c1) (fun x -> (morph (wp2 x) (c2 x))))) =
+                  on_wp c (morph wp c) == on_wp c (lbind (morph wp1 c1) (fun x -> (morph (wp2 x) (c2 x)))))) =
   let p = bind_inv c1 c2 c in
   assert (subsumes (bind_wp wp1 wp2) wp);
   assert (l_eq #b
@@ -577,7 +588,7 @@ let morph_for (wp1 : int -> hwp_mon unit) (lo : int) (hi : int{lo <= hi}) (f : (
     (wp : hwp_mon unit) (c : comp_wp unit wp) :
   Lemma (requires (c === for_elab lo hi f))
         (ensures (for_inv lo hi f c;
-                  morph wp c == lfor lo hi (fun i -> morph (wp1 i) (f i)))) =
+                  on_wp c (morph wp c) == on_wp c (lfor lo hi (fun i -> morph (wp1 i) (f i))))) =
   let p = for_inv lo hi f c in
   assert (subsumes (for_wp wp1 lo hi) wp);
   assert (l_eq #unit
@@ -597,7 +608,7 @@ let morph_for' (inv : state -> int -> Type0) (f : (i:int) -> comp_p unit (fun h0
                (wp : hwp_mon unit) (c : comp_wp unit wp) :
   Lemma (requires (c === for_elab' inv f lo hi))
         (ensures (for_inv' inv f lo hi c;
-                  morph wp c == lfor' inv f (fun i -> morph _ (f i)) lo hi)) =
+                  on_wp c (morph wp c) == on_wp c (lfor' inv f (fun i -> morph _ (f i)) lo hi))) =
   let p = for_inv' inv f lo hi c in
   assert (l_eq #unit
                #wp #(cast wp (for_elab' inv f lo hi)) (morph wp (cast wp (for_elab' inv f lo hi)))
@@ -616,7 +627,7 @@ let morph_ite #a (b : bool) (wp1 : hwp_mon a) (c1 : comp_wp a wp1)
     (wp : hwp_mon a) (c : comp_wp a wp):
   Lemma (requires (c === ite_elab b c1 c2))
         (ensures (ite_inv b c1 c2 c;
-                  morph wp c == lite b (morph wp1 c1) (morph wp2 c2))) =
+                  on_wp c (morph wp c) == on_wp c (lite b (morph wp1 c1) (morph wp2 c2)))) =
   let p = ite_inv b c1 c2 c in
   assert (subsumes (ite_wp b wp1 wp2) wp);
   assert (l_eq #a
